feat(data/list/basic): erasep

data/list/basic.lean
@@ -1799,7 +1799,7 @@ begin
   { rw [filter_cons_of_pos _ h, cons_inj', ih, and_iff_right h] },
   { rw [filter_cons_of_neg _ h],
     refine iff_of_false _ (mt and.left h), intro e,
-    have := filter_sublist l, rw e at this,
+  have := filter_sublist l, rw e at this,
     exact not_lt_of_ge (length_le_of_sublist this) (lt_succ_self _) }
 end
 
@@ -2642,7 +2642,7 @@ by simp only [insert.def, if_neg h]; split; refl
 begin
   by_cases h' : b ∈ l,
   { simp only [insert_of_mem h'],
-    apply (or_iff_right_of_imp _).symm,
+  apply (or_iff_right_of_imp _).symm,
     exact λ e, e.symm ▸ h' },
   simp only [insert_of_not_mem h', mem_cons_iff]
 end
@@ -2669,6 +2669,106 @@ by rw insert_of_not_mem h; refl
 
 end insert
 
+/- erasep -/
+section erasep
+variables {p : α → Prop} [decidable_pred p]
+
+def erasep (p : α → Prop) [decidable_pred p] : list α → list α
+| []     := []
+| (a::l) := if p a then l else a :: erasep l
+
+@[simp] theorem erasep_nil : [].erasep p = [] := rfl
+
+theorem erasep_cons (a : α) (l : list α) : (a :: l).erasep p = if p a then l else a :: l.erasep p := rfl
+
+@[simp] theorem erasep_cons_of_pos {a : α} {l : list α} (h : p a) : (a :: l).erasep p = l :=
+by simp [erasep_cons, h]
+
+@[simp] theorem erasep_cons_of_neg {a : α} {l : list α} (h : ¬ p a) : (a::l).erasep p = a :: l.erasep p :=
+by simp [erasep_cons, h]
+
+theorem erasep_of_forall_not {l : list α}
+  (h : ∀ a ∈ l, ¬ p a) : l.erasep p = l :=
+by induction l with _ _ ih; [refl,
+  simp [h _ (or.inl rfl), ih (forall_mem_of_forall_mem_cons h)]]
+
+theorem exists_of_erasep {l : list α} {a} (al : a ∈ l) (pa : p a) :
+  ∃ a l₁ l₂, (∀ b ∈ l₁, ¬ p b) ∧ p a ∧ l = l₁ ++ a :: l₂ ∧ l.erasep p = l₁ ++ l₂ :=
+begin
+  induction l with b l IH, {cases al},
+  by_cases pb : p b,
+  { exact ⟨b, [], l, forall_mem_nil _, pb, by simp [pb]⟩ },
+  { rcases al with rfl | al, {exact pb.elim pa},
+    rcases IH al with ⟨c, l₁, l₂, h₁, h₂, h₃, h₄⟩,
+    exact ⟨c, b::l₁, l₂, forall_mem_cons.2 ⟨pb, h₁⟩,
+      h₂, by rw h₃; refl, by simp [pb, h₄]⟩ }
+end
+
+theorem exists_or_eq_self_of_erasep (l : list α) :
+  l.erasep p = l ∨ ∃ a l₁ l₂, (∀ b ∈ l₁, ¬ p b) ∧ p a ∧ l = l₁ ++ a :: l₂ ∧ l.erasep p = l₁ ++ l₂ :=
+begin
+  by_cases h : ∃ a ∈ l, p a,
+  { rcases h with ⟨a, ha, pa⟩,
+    exact or.inr (exists_of_erasep ha pa) },
+  { simp at h, exact or.inl (erasep_of_forall_not h) }
+end
+
+@[simp] theorem length_erasep_of_mem {l : list α} {a} (al : a ∈ l) (pa : p a) :
+ length (l.erasep p) = pred (length l) :=
+by rcases exists_of_erasep al pa with ⟨_, l₁, l₂, _, _, e₁, e₂⟩;
+   rw e₂; simp [-add_comm, e₁]; refl
+
+theorem erasep_append_left {a : α} (pa : p a) :
+  ∀ {l₁ : list α} (l₂), a ∈ l₁ → (l₁++l₂).erasep p = l₁.erasep p ++ l₂
+| (x::xs) l₂ h := begin
+  by_cases h' : p x; simp [h'],
+  rw erasep_append_left l₂ (mem_of_ne_of_mem (mt _ h') h),
+  rintro rfl, exact pa
+end
+
+theorem erasep_append_right : ∀ {l₁ : list α} (l₂), (∀ b ∈ l₁, ¬ p b) → (l₁++l₂).erasep p = l₁ ++ l₂.erasep p
+| []      l₂ h := rfl
+| (x::xs) l₂ h := by simp [(forall_mem_cons.1 h).1,
+  erasep_append_right _ (forall_mem_cons.1 h).2]
+
+theorem erasep_sublist (l : list α) : l.erasep p <+ l :=
+by rcases exists_or_eq_self_of_erasep l with h | ⟨c, l₁, l₂, h₁, h₂, h₃, h₄⟩;
+   [rw h, {rw [h₄, h₃], simp}]
+
+theorem erasep_subset (l : list α) : l.erasep p ⊆ l :=
+subset_of_sublist (erasep_sublist l)
+
+theorem erasep_sublist_erasep {l₁ l₂ : list α} (s : l₁ <+ l₂) : l₁.erasep p <+ l₂.erasep p :=
+begin
+  induction s,
+  case list.sublist.slnil { refl },
+  case list.sublist.cons : l₁ l₂ a s IH {
+    by_cases h : p a; simp [h],
+    exacts [IH.trans (erasep_sublist _), IH.cons _ _ _] },
+  case list.sublist.cons2 : l₁ l₂ a s IH {
+    by_cases h : p a; simp [h],
+    exacts [s, IH.cons2 _ _ _] }
+end
+
+theorem mem_of_mem_erasep {a : α} {l : list α} : a ∈ l.erasep p → a ∈ l :=
+@erasep_subset _ _ _ _ _
+
+@[simp] theorem mem_erasep_of_neg {a : α} {l : list α} (pa : ¬ p a) : a ∈ l.erasep p ↔ a ∈ l :=
+⟨mem_of_mem_erasep, λ al, begin
+  rcases exists_or_eq_self_of_erasep l with h | ⟨c, l₁, l₂, h₁, h₂, h₃, h₄⟩,
+  { rwa h },
+  { rw h₄, rw h₃ at al,
+    have : a ≠ c, {rintro rfl, exact pa.elim h₂},
+    simpa [this] using al }
+end⟩
+
+theorem erasep_map [decidable_eq β] (f : β → α) :
+  ∀ (l : list β), (map f l).erasep p = map f (l.erasep (p ∘ f))
+| []     := rfl
+| (b::l) := by by_cases p (f b); simp [h, erasep_map l]
+
+end erasep
+
 /- erase -/
 section erase
 variable [decidable_eq α]
@@ -2683,60 +2783,44 @@ by simp only [erase_cons, if_pos rfl]
 @[simp] theorem erase_cons_tail {a b : α} (l : list α) (h : b ≠ a) : (b::l).erase a = b :: l.erase a :=
 by simp only [erase_cons, if_neg h]; split; refl
 
+theorem erase_eq_erasep (a : α) (l : list α) : l.erase a = l.erasep (eq a) :=
+by { induction l with b l, {refl},
+  by_cases a = b; [simp [h], simp [h, ne.symm h, *]] }
+
 @[simp] theorem erase_of_not_mem {a : α} {l : list α} (h : a ∉ l) : l.erase a = l :=
-by induction l with _ _ ih; [refl,
-  simp only [list.erase, if_neg (ne_of_not_mem_cons h).symm, ih (not_mem_of_not_mem_cons h)]]; split; refl
+by rw [erase_eq_erasep, erasep_of_forall_not]; rintro b h' rfl; exact h h'
 
 theorem exists_erase_eq {a : α} {l : list α} (h : a ∈ l) :
   ∃ l₁ l₂, a ∉ l₁ ∧ l = l₁ ++ a :: l₂ ∧ l.erase a = l₁ ++ l₂ :=
-by induction l with b l ih; [cases h, {
-  by_cases e : b = a,
-  { subst b, exact ⟨[], l, not_mem_nil _, rfl, by simp only [erase_cons_head, nil_append]⟩ },
-  { exact let ⟨l₁, l₂, h₁, h₂, h₃⟩ := ih (h.resolve_left (ne.symm e)) in
-    ⟨b::l₁, l₂, not_mem_cons_of_ne_of_not_mem (ne.symm e) h₁,
-      by rw h₂; refl,
-      by simp only [erase_cons_tail _ e, h₃, cons_append]; split; refl⟩ } }]
+by rcases exists_of_erasep h rfl with ⟨_, l₁, l₂, h₁, rfl, h₂, h₃⟩;
+   rw erase_eq_erasep; exact ⟨l₁, l₂, λ h, h₁ _ h rfl, h₂, h₃⟩
 
 @[simp] theorem length_erase_of_mem {a : α} {l : list α} (h : a ∈ l) : length (l.erase a) = pred (length l) :=
-match l, l.erase a, exists_erase_eq h with
-| ._, ._, ⟨l₁, l₂, _, rfl, rfl⟩ := by simp only [length_append]; refl
-end
+by rw erase_eq_erasep; exact length_erasep_of_mem h rfl
 
-theorem erase_append_left {a : α} : ∀ {l₁ : list α} (l₂), a ∈ l₁ → (l₁++l₂).erase a = l₁.erase a ++ l₂
-| (x::xs) l₂  h := begin
-  by_cases h' : x = a, { simp only [h', erase_cons_head, cons_append] },
-  simp only [cons_append, erase_cons_tail _ h', erase_append_left l₂ (mem_of_ne_of_mem (ne.symm h') h)], split; refl
-end
+theorem erase_append_left {a : α} {l₁ : list α} (l₂) (h : a ∈ l₁) :
+  (l₁++l₂).erase a = l₁.erase a ++ l₂ :=
+by simp [erase_eq_erasep]; exact erasep_append_left (by refl) l₂ h
 
-theorem erase_append_right {a : α} : ∀ {l₁ : list α} (l₂), a ∉ l₁ → (l₁++l₂).erase a = l₁ ++ l₂.erase a
-| []      l₂ h := rfl
-| (x::xs) l₂ h := by simp only [*, cons_append, erase_cons_tail _(ne_of_not_mem_cons h).symm, erase_append_right _ (not_mem_of_not_mem_cons h)]; split; refl
+theorem erase_append_right {a : α} {l₁ : list α} (l₂) (h : a ∉ l₁) :
+  (l₁++l₂).erase a = l₁ ++ l₂.erase a :=
+by rw [erase_eq_erasep, erase_eq_erasep, erasep_append_right];
+   rintro b h' rfl; exact h h'
 
 theorem erase_sublist (a : α) (l : list α) : l.erase a <+ l :=
-if h : a ∈ l then match l, l.erase a, exists_erase_eq h with
-| ._, ._, ⟨l₁, l₂, _, rfl, rfl⟩ := by simp only [append_sublist_append_left, sublist_cons]
-end else by rw erase_of_not_mem h
+by rw erase_eq_erasep; apply erasep_sublist
 
 theorem erase_subset (a : α) (l : list α) : l.erase a ⊆ l :=
 subset_of_sublist (erase_sublist a l)
 
-theorem erase_sublist_erase (a : α) : ∀ {l₁ l₂ : list α}, l₁ <+ l₂ → l₁.erase a <+ l₂.erase a
-| ._ ._ sublist.slnil             := sublist.slnil
-| ._ ._ (sublist.cons  l₁ l₂ b s) := if h : b = a
-  then by rw [h, erase_cons_head]; exact (erase_sublist _ _).trans s
-  else by rw erase_cons_tail _ h; exact (erase_sublist_erase s).cons _ _ _
-| ._ ._ (sublist.cons2 l₁ l₂ b s) := if h : b = a
-  then by rw [h, erase_cons_head, erase_cons_head]; exact s
-  else by rw [erase_cons_tail _ h, erase_cons_tail _ h]; exact (erase_sublist_erase s).cons2 _ _ _
+theorem erase_sublist_erase (a : α) {l₁ l₂ : list α} (h : l₁ <+ l₂) : l₁.erase a <+ l₂.erase a :=
+by simp [erase_eq_erasep]; exact erasep_sublist_erasep h
 
 theorem mem_of_mem_erase {a b : α} {l : list α} : a ∈ l.erase b → a ∈ l :=
 @erase_subset _ _ _ _ _
 
 @[simp] theorem mem_erase_of_ne {a b : α} {l : list α} (ab : a ≠ b) : a ∈ l.erase b ↔ a ∈ l :=
-⟨mem_of_mem_erase, λ al,
-  if h : b ∈ l then match l, l.erase b, exists_erase_eq h, al with
-  | ._, ._, ⟨l₁, l₂, _, rfl, rfl⟩, al := by simpa only [mem_append, mem_cons_iff, ab, false_or] using al
-  end else by simp only [erase_of_not_mem h, al]⟩
+by rw erase_eq_erasep; exact mem_erasep_of_neg ab.symm
 
 theorem erase_comm (a b : α) (l : list α) : (l.erase a).erase b = (l.erase b).erase a :=
 if ab : a = b then by rw ab else
